MapFunction.dfy
@@ -54,237 +54,237 @@ module MapFunction {
     && |so.state| == |state|
   }
 
-  datatype MapFunction = MapFunction(
-    inputs: seq<NP>,
-    outputs: seq<NP>,
-    state: seq<CNode>,
-    sf: SI --> SO
-  ) {
+  //datatype MapFunction = MapFunction(
+  //  inputs: seq<NP>,
+  //  outputs: seq<NP>,
+  //  state: seq<CNode>,
+  //  sf: SI --> SO
+  //) {
 
-    ghost opaque predicate Valid()
-    {
-      && (forall si: SI :: SIValid(si, inputs, state) ==> (
-          && sf.requires(si)
-          && SOValid(sf(si), outputs, state)
-      ))
-      && Seq.HasNoDuplicates(inputs)
-      && Seq.HasNoDuplicates(outputs)
-      && Seq.HasNoDuplicates(state)
-      && SeqsNoIntersection(inputs, outputs)
-      && SeqsNoIntersection(inputs, StateONPsSeq(state))
-      && SeqsNoIntersection(outputs, StateINPsSeq(state))
-    }
+  //  ghost opaque predicate Valid()
+  //  {
+  //    && (forall si: SI :: SIValid(si, inputs, state) ==> (
+  //        && sf.requires(si)
+  //        && SOValid(sf(si), outputs, state)
+  //    ))
+  //    && Seq.HasNoDuplicates(inputs)
+  //    && Seq.HasNoDuplicates(outputs)
+  //    && Seq.HasNoDuplicates(state)
+  //    && SeqsNoIntersection(inputs, outputs)
+  //    && SeqsNoIntersection(inputs, StateONPsSeq(state))
+  //    && SeqsNoIntersection(outputs, StateINPsSeq(state))
+  //  }
 
-    function NPs(): set<NP>
-    {
-      Seq.ToSet(inputs) + Seq.ToSet(outputs) + StateONPs(state) + StateINPs(state)
-    }
+  //  function NPs(): set<NP>
+  //  {
+  //    Seq.ToSet(inputs) + Seq.ToSet(outputs) + StateONPs(state) + StateINPs(state)
+  //  }
 
-    function rf(): (r: RFunction)
-      requires Valid()
-      ensures r.Valid()
-    {
-      reveal MapFunction.Valid();
-      reveal RFunction.Valid();
-      RFunction(|inputs|, |outputs|, |state|, sf)
-    }
+  //  function rf(): (r: UpdateFunction)
+  //    requires Valid()
+  //    ensures r.Valid()
+  //  {
+  //    reveal MapFunction.Valid();
+  //    reveal UpdateFunction.Valid();
+  //    UpdateFunction(|inputs|, |outputs|, |state|, sf)
+  //  }
 
-    lemma InputsHasNoDuplicates()
-      requires Valid()
-      ensures Seq.HasNoDuplicates(inputs)
-    {
-      reveal Valid();
-    }
+  //  lemma InputsHasNoDuplicates()
+  //    requires Valid()
+  //    ensures Seq.HasNoDuplicates(inputs)
+  //  {
+  //    reveal Valid();
+  //  }
 
-    lemma OutputsHasNoDuplicates()
-      requires Valid()
-      ensures Seq.HasNoDuplicates(outputs)
-    {
-      reveal Valid();
-    }
+  //  lemma OutputsHasNoDuplicates()
+  //    requires Valid()
+  //    ensures Seq.HasNoDuplicates(outputs)
+  //  {
+  //    reveal Valid();
+  //  }
 
-    function si2fi(si: SI): (fi: FI)
-      requires SIValid(si, inputs, state)
-      ensures FIValid(fi, inputs, state)
-    {
-      reveal Seq.HasNoDuplicates();
-      var i := SeqsToMap(inputs, si.inputs);
-      assert i.Keys == Seq.ToSet(inputs);
-      var s := SeqsToMap(state, si.state);
-      FI(i, s)
-    }
-    
-    function so2fo(so: SO): (fo: FO)
-      requires SOValid(so, outputs, state)
-      ensures FOValid(fo, outputs, state)
-    {
-      var o := SeqsToMap(outputs, so.outputs);
-      var s := SeqsToMap(state, so.state);
-      FO(o, s)
-    }
+  //  function si2fi(si: SI): (fi: FI)
+  //    requires SIValid(si, inputs, state)
+  //    ensures FIValid(fi, inputs, state)
+  //  {
+  //    reveal Seq.HasNoDuplicates();
+  //    var i := SeqsToMap(inputs, si.inputs);
+  //    assert i.Keys == Seq.ToSet(inputs);
+  //    var s := SeqsToMap(state, si.state);
+  //    FI(i, s)
+  //  }
+  //  
+  //  function so2fo(so: SO): (fo: FO)
+  //    requires SOValid(so, outputs, state)
+  //    ensures FOValid(fo, outputs, state)
+  //  {
+  //    var o := SeqsToMap(outputs, so.outputs);
+  //    var s := SeqsToMap(state, so.state);
+  //    FO(o, s)
+  //  }
 
-    function fo2so(fo: FO): (so: SO)
-      requires Valid()
-      requires FOValid(fo, outputs, state)
-      ensures SOValid(so, outputs, state)
-    {
-      var o := seq(|outputs|, (index: nat) requires index < |outputs| =>
-        reveal Seq.ToSet();
-        fo.outputs[outputs[index]]);
-      var s := seq(|state|, (index: nat) requires index < |state| =>
-        reveal Seq.ToSet();
-        fo.state[state[index]]);
-      reveal Valid();
-      reveal Seq.HasNoDuplicates();
-      OutputsHasNoDuplicates();
-      SO(o, s)
-    }
+  //  function fo2so(fo: FO): (so: SO)
+  //    requires Valid()
+  //    requires FOValid(fo, outputs, state)
+  //    ensures SOValid(so, outputs, state)
+  //  {
+  //    var o := seq(|outputs|, (index: nat) requires index < |outputs| =>
+  //      reveal Seq.ToSet();
+  //      fo.outputs[outputs[index]]);
+  //    var s := seq(|state|, (index: nat) requires index < |state| =>
+  //      reveal Seq.ToSet();
+  //      fo.state[state[index]]);
+  //    reveal Valid();
+  //    reveal Seq.HasNoDuplicates();
+  //    OutputsHasNoDuplicates();
+  //    SO(o, s)
+  //  }
 
-    function fi2si(fi: FI): (si: SI)
-      requires Valid()
-      requires FIValid(fi, inputs, state)
-      ensures SIValid(si, inputs, state)
-    {
-      var i := seq(|inputs|, (index: nat) requires index < |inputs| =>
-        reveal Seq.ToSet();
-        fi.inputs[inputs[index]]);
-      var s := seq(|state|, (index: nat) requires index < |state| =>
-        reveal Seq.ToSet();
-        fi.state[state[index]]);
-      reveal Valid();
-      reveal Seq.HasNoDuplicates();
-      InputsHasNoDuplicates();
-      SI(i, s)
-    }
+  //  function fi2si(fi: FI): (si: SI)
+  //    requires Valid()
+  //    requires FIValid(fi, inputs, state)
+  //    ensures SIValid(si, inputs, state)
+  //  {
+  //    var i := seq(|inputs|, (index: nat) requires index < |inputs| =>
+  //      reveal Seq.ToSet();
+  //      fi.inputs[inputs[index]]);
+  //    var s := seq(|state|, (index: nat) requires index < |state| =>
+  //      reveal Seq.ToSet();
+  //      fi.state[state[index]]);
+  //    reveal Valid();
+  //    reveal Seq.HasNoDuplicates();
+  //    InputsHasNoDuplicates();
+  //    SI(i, s)
+  //  }
 
-    lemma fi2si2fi(fi: FI)
-      requires Valid()
-      requires FIValid(fi, inputs, state)
-      ensures si2fi(fi2si(fi)) == fi
-    {
-      var si := fi2si(fi);
-      assert si.inputs == seq(|inputs|, (index: nat) requires index < |inputs| =>
-        reveal Seq.ToSet();
-        fi.inputs[inputs[index]]);
-      var fi_next := si2fi(si);
-      assert fi_next.inputs == SeqsToMap(inputs, si.inputs);
-      forall np | np in fi.inputs
-        ensures fi_next.inputs[np] == fi.inputs[np]
-      {
-        reveal Seq.ToSet();
-        assert np in inputs;
-        var index := Seq.IndexOf(inputs, np);
-        assert si.inputs[index] == fi.inputs[np];
-        reveal MapMatchesSeqs();
-        reveal SeqsToMap();
-        assert fi_next.inputs[np] == si.inputs[index];
-      }
-      assert fi_next.inputs == fi.inputs;
+  //  lemma fi2si2fi(fi: FI)
+  //    requires Valid()
+  //    requires FIValid(fi, inputs, state)
+  //    ensures si2fi(fi2si(fi)) == fi
+  //  {
+  //    var si := fi2si(fi);
+  //    assert si.inputs == seq(|inputs|, (index: nat) requires index < |inputs| =>
+  //      reveal Seq.ToSet();
+  //      fi.inputs[inputs[index]]);
+  //    var fi_next := si2fi(si);
+  //    assert fi_next.inputs == SeqsToMap(inputs, si.inputs);
+  //    forall np | np in fi.inputs
+  //      ensures fi_next.inputs[np] == fi.inputs[np]
+  //    {
+  //      reveal Seq.ToSet();
+  //      assert np in inputs;
+  //      var index := Seq.IndexOf(inputs, np);
+  //      assert si.inputs[index] == fi.inputs[np];
+  //      reveal MapMatchesSeqs();
+  //      reveal SeqsToMap();
+  //      assert fi_next.inputs[np] == si.inputs[index];
+  //    }
+  //    assert fi_next.inputs == fi.inputs;
 
-      assert fi_next.state == SeqsToMap(state, si.state);
-      forall n | n in fi.state
-        ensures fi_next.state[n] == fi.state[n]
-      {
-        reveal Seq.ToSet();
-        assert n in state;
-        var index := Seq.IndexOf(state, n);
-        assert si.state[index] == fi.state[n];
-        reveal MapMatchesSeqs();
-        reveal SeqsToMap();
-        assert fi_next.state[n] == si.state[index];
-      }
-      assert fi_next.inputs == fi.inputs;
-    }
+  //    assert fi_next.state == SeqsToMap(state, si.state);
+  //    forall n | n in fi.state
+  //      ensures fi_next.state[n] == fi.state[n]
+  //    {
+  //      reveal Seq.ToSet();
+  //      assert n in state;
+  //      var index := Seq.IndexOf(state, n);
+  //      assert si.state[index] == fi.state[n];
+  //      reveal MapMatchesSeqs();
+  //      reveal SeqsToMap();
+  //      assert fi_next.state[n] == si.state[index];
+  //    }
+  //    assert fi_next.inputs == fi.inputs;
+  //  }
 
-    lemma fo2so2fo(fo: FO)
-      requires Valid()
-      requires FOValid(fo, outputs, state)
-      ensures so2fo(fo2so(fo)) == fo
-    {
-      var so := fo2so(fo);
-      assert so.outputs == seq(|outputs|, (index: nat) requires index < |outputs| =>
-        reveal Seq.ToSet();
-        fo.outputs[outputs[index]]);
-      var fo_next := so2fo(so);
-      assert fo_next.outputs == SeqsToMap(outputs, so.outputs);
-      forall np | np in fo.outputs
-        ensures fo_next.outputs[np] == fo.outputs[np]
-      {
-        reveal Seq.ToSet();
-        assert np in outputs;
-        var index := Seq.IndexOf(outputs, np);
-        assert so.outputs[index] == fo.outputs[np];
-        reveal MapMatchesSeqs();
-        reveal SeqsToMap();
-        assert fo_next.outputs[np] == so.outputs[index];
-      }
-      assert fo_next.outputs == fo.outputs;
+  //  lemma fo2so2fo(fo: FO)
+  //    requires Valid()
+  //    requires FOValid(fo, outputs, state)
+  //    ensures so2fo(fo2so(fo)) == fo
+  //  {
+  //    var so := fo2so(fo);
+  //    assert so.outputs == seq(|outputs|, (index: nat) requires index < |outputs| =>
+  //      reveal Seq.ToSet();
+  //      fo.outputs[outputs[index]]);
+  //    var fo_next := so2fo(so);
+  //    assert fo_next.outputs == SeqsToMap(outputs, so.outputs);
+  //    forall np | np in fo.outputs
+  //      ensures fo_next.outputs[np] == fo.outputs[np]
+  //    {
+  //      reveal Seq.ToSet();
+  //      assert np in outputs;
+  //      var index := Seq.IndexOf(outputs, np);
+  //      assert so.outputs[index] == fo.outputs[np];
+  //      reveal MapMatchesSeqs();
+  //      reveal SeqsToMap();
+  //      assert fo_next.outputs[np] == so.outputs[index];
+  //    }
+  //    assert fo_next.outputs == fo.outputs;
 
-      assert fo_next.state == SeqsToMap(state, so.state);
-      forall n | n in fo.state
-        ensures fo_next.state[n] == fo.state[n]
-      {
-        reveal Seq.ToSet();
-        assert n in state;
-        var index := Seq.IndexOf(state, n);
-        assert so.state[index] == fo.state[n];
-        reveal MapMatchesSeqs();
-        reveal SeqsToMap();
-        assert fo_next.state[n] == so.state[index];
-      }
-      assert fo_next.outputs == fo.outputs;
-    }
+  //    assert fo_next.state == SeqsToMap(state, so.state);
+  //    forall n | n in fo.state
+  //      ensures fo_next.state[n] == fo.state[n]
+  //    {
+  //      reveal Seq.ToSet();
+  //      assert n in state;
+  //      var index := Seq.IndexOf(state, n);
+  //      assert so.state[index] == fo.state[n];
+  //      reveal MapMatchesSeqs();
+  //      reveal SeqsToMap();
+  //      assert fo_next.state[n] == so.state[index];
+  //    }
+  //    assert fo_next.outputs == fo.outputs;
+  //  }
 
-    lemma si2fi2si(si: SI)
-      requires Valid()
-      requires SIValid(si, inputs, state)
-      ensures fi2si(si2fi(si)) == si
-    {
-      reveal MapMatchesSeqs();
-      reveal SeqsToMap();
-    }
+  //  lemma si2fi2si(si: SI)
+  //    requires Valid()
+  //    requires SIValid(si, inputs, state)
+  //    ensures fi2si(si2fi(si)) == si
+  //  {
+  //    reveal MapMatchesSeqs();
+  //    reveal SeqsToMap();
+  //  }
 
-    lemma so2fo2so(so: SO)
-      requires Valid()
-      requires SOValid(so, outputs, state)
-      ensures fo2so(so2fo(so)) == so
-    {
-      reveal MapMatchesSeqs();
-      reveal SeqsToMap();
-    }
+  //  lemma so2fo2so(so: SO)
+  //    requires Valid()
+  //    requires SOValid(so, outputs, state)
+  //    ensures fo2so(so2fo(so)) == so
+  //  {
+  //    reveal MapMatchesSeqs();
+  //    reveal SeqsToMap();
+  //  }
 
-    function f(fi: FI): (fo: FO)
-      requires Valid()
-      requires FIValid(fi, inputs, state)
-      ensures FOValid(fo, outputs, state)
-    {
-      var si := fi2si(fi);
-      assert SIValid(si, inputs, state);
-      reveal Valid();
-      var so := sf(si);
-      var fo := so2fo(so);
-      fo
-    }
+  //  function f(fi: FI): (fo: FO)
+  //    requires Valid()
+  //    requires FIValid(fi, inputs, state)
+  //    ensures FOValid(fo, outputs, state)
+  //  {
+  //    var si := fi2si(fi);
+  //    assert SIValid(si, inputs, state);
+  //    reveal Valid();
+  //    var so := sf(si);
+  //    var fo := so2fo(so);
+  //    fo
+  //  }
 
-    lemma NotInBothOutputsAndStateINPs(np: NP)
-      requires Valid()
-      ensures !(np in outputs && np in StateINPs(state))
-    {
-      reveal Valid();
-      StateINPsSeqSame(state);
-      reveal Seq.ToSet();
-    }
+  //  lemma NotInBothOutputsAndStateINPs(np: NP)
+  //    requires Valid()
+  //    ensures !(np in outputs && np in StateINPs(state))
+  //  {
+  //    reveal Valid();
+  //    StateINPsSeqSame(state);
+  //    reveal Seq.ToSet();
+  //  }
 
-    lemma NotInBothInputsAndStateONPs(np: NP)
-      requires Valid()
-      ensures !(np in inputs && np in StateONPs(state))
-    {
-      reveal Valid();
-      StateONPsSeqSame(state);
-      reveal Seq.ToSet();
-    }
+  //  lemma NotInBothInputsAndStateONPs(np: NP)
+  //    requires Valid()
+  //    ensures !(np in inputs && np in StateONPs(state))
+  //  {
+  //    reveal Valid();
+  //    StateONPsSeqSame(state);
+  //    reveal Seq.ToSet();
+  //  }
 
-  }
+  //}
 
   function StateINPsSeq(state: seq<CNode>): seq<NP>
   {
@@ -393,101 +393,253 @@ module MapFunction {
     (set n | n in state :: NP(n, OUTPUT_0))
   }
 
-  function MFLookupOutput(mf: MapFunction, fi: FI, np: NP): bool
-    requires mf.Valid()
-    requires FIValid(fi, mf.inputs, mf.state)
-    requires np in mf.outputs
-  {
-    reveal mf.Valid();
-    var fo := mf.f(fi);
-    assert FOValid(fo, mf.outputs, mf.state);
-    reveal Seq.ToSet();
-    fo.outputs[np]
-  }
-
-  function MFLookupState(mf: MapFunction, fi: FI, np: NP): bool
-    requires mf.Valid()
-    requires FIValid(fi, mf.inputs, mf.state)
-    requires np in StateINPs(mf.state)
-  {
-    reveal mf.Valid();
-    var fo := mf.f(fi);
-    assert FOValid(fo, mf.outputs, mf.state);
-    reveal Seq.ToSet();
-    fo.state[np.n]
-  }
-
-  function MFLookup(mf: MapFunction, fi: FI, np: NP): bool
-    requires mf.Valid()
-    requires FIValid(fi, mf.inputs, mf.state)
-    requires np in mf.outputs || np in StateINPs(mf.state)
-  {
-    assert !((np in mf.outputs) && (np in StateINPs(mf.state))) by {
-      reveal mf.Valid();
-      reveal Seq.ToSet();
-      StateINPsSeqSame(mf.state);
-    }
-    if (np in mf.outputs) then
-      MFLookupOutput(mf, fi, np)
-    else
-      MFLookupState(mf, fi, np)
-  }
-
-  opaque ghost predicate MapFunctionsEquiv(mf1: MapFunction, mf2: MapFunction)
-    requires mf1.Valid()
-    requires mf2.Valid()
-  {
-    reveal MapFunction.Valid();
-    && mf1.inputs == mf2.inputs
-    && mf1.outputs == mf2.outputs
-    && mf1.state == mf2.state
-    && forall fi: FI :: FIValid(fi, mf1.inputs, mf1.state) ==> (
-      mf1.f(fi) == mf2.f(fi)
-    )
-  }
-
-  opaque ghost predicate MapFunctionsSFEquiv(mf1: MapFunction, mf2: MapFunction)
-    requires mf1.Valid()
-    requires mf2.Valid()
-  {
-    reveal MapFunction.Valid();
-    && mf1.inputs == mf2.inputs
-    && mf1.outputs == mf2.outputs
-    && mf1.state == mf2.state
-    && forall si: SI :: SIValid(si, mf1.inputs, mf1.state) ==> (
-      mf1.sf(si) == mf2.sf(si)
-    )
-  }
-
-  lemma MapFunctionsEquivSFEquiv(mf1: MapFunction, mf2: MapFunction)
-    requires mf1.Valid()
-    requires mf2.Valid()
-    requires MapFunctionsSFEquiv(mf1, mf2)
-    ensures MapFunctionsEquiv(mf1, mf2)
-  {
-    reveal MapFunctionsSFEquiv();
-    reveal MapFunction.Valid();
-    forall fi: FI | FIValid(fi, mf1.inputs, mf1.state)
-      ensures mf1.f(fi) == mf2.f(fi)
+  datatype ScufMap = ScufMap(
+    inputs: seq<NP>,
+    outputs: seq<NP>,
+    state: seq<CNode>
+  ) {
+    ghost predicate Valid()
     {
-      var si1 := mf1.fi2si(fi);
-      var si2 := mf2.fi2si(fi);
-      mf1.fi2si2fi(fi);
-      mf2.fi2si2fi(fi);
-      assert si1 == si2;
-      var so1 := mf1.sf(si1);
-      var so2 := mf2.sf(si2);
-      assert so1 == so2;
-      var fo1 := mf1.f(fi);
-      var fo2 := mf2.f(fi);
-      assert fo1 == mf1.so2fo(so1);
-      assert fo2 == mf2.so2fo(so2);
-      assert fo1 == fo2;
+      && Seq.HasNoDuplicates(inputs)
+      && Seq.HasNoDuplicates(outputs)
+      && Seq.HasNoDuplicates(state)
+      && SeqsNoIntersection(inputs, outputs)
+      && SeqsNoIntersection(inputs, StateONPsSeq(state))
+      && SeqsNoIntersection(outputs, StateINPsSeq(state))
     }
-    reveal MapFunctionsEquiv();
+
+    function NPs(): set<NP>
+    {
+      Seq.ToSet(inputs) + Seq.ToSet(outputs) + StateONPs(state) + StateINPs(state)
+    }
+
+    function si2fi(si: SI): (fi: FI)
+      requires SIValid(si, inputs, state)
+      ensures FIValid(fi, inputs, state)
+    {
+      reveal Seq.HasNoDuplicates();
+      var i := SeqsToMap(inputs, si.inputs);
+      assert i.Keys == Seq.ToSet(inputs);
+      var s := SeqsToMap(state, si.state);
+      FI(i, s)
+    }
+    
+    function so2fo(so: SO): (fo: FO)
+      requires SOValid(so, outputs, state)
+      ensures FOValid(fo, outputs, state)
+    {
+      var o := SeqsToMap(outputs, so.outputs);
+      var s := SeqsToMap(state, so.state);
+      FO(o, s)
+    }
+
+    function fo2so(fo: FO): (so: SO)
+      requires Valid()
+      requires FOValid(fo, outputs, state)
+      ensures SOValid(so, outputs, state)
+    {
+      var o := seq(|outputs|, (index: nat) requires index < |outputs| =>
+        reveal Seq.ToSet();
+        fo.outputs[outputs[index]]);
+      var s := seq(|state|, (index: nat) requires index < |state| =>
+        reveal Seq.ToSet();
+        fo.state[state[index]]);
+      reveal Seq.HasNoDuplicates();
+      SO(o, s)
+    }
+
+    function fi2si(fi: FI): (si: SI)
+      requires Valid()
+      requires FIValid(fi, inputs, state)
+      ensures SIValid(si, inputs, state)
+    {
+      var i := seq(|inputs|, (index: nat) requires index < |inputs| =>
+        reveal Seq.ToSet();
+        fi.inputs[inputs[index]]);
+      var s := seq(|state|, (index: nat) requires index < |state| =>
+        reveal Seq.ToSet();
+        fi.state[state[index]]);
+      //reveal Valid();
+      reveal Seq.HasNoDuplicates();
+      //InputsHasNoDuplicates();
+      SI(i, s)
+    }
+
+    lemma fi2si2fi(fi: FI)
+      requires Valid()
+      requires FIValid(fi, inputs, state)
+      ensures si2fi(fi2si(fi)) == fi
+    {
+      var si := fi2si(fi);
+      assert si.inputs == seq(|inputs|, (index: nat) requires index < |inputs| =>
+        reveal Seq.ToSet();
+        fi.inputs[inputs[index]]);
+      var fi_next := si2fi(si);
+      assert fi_next.inputs == SeqsToMap(inputs, si.inputs);
+      forall np | np in fi.inputs
+        ensures fi_next.inputs[np] == fi.inputs[np]
+      {
+        reveal Seq.ToSet();
+        assert np in inputs;
+        var index := Seq.IndexOf(inputs, np);
+        assert si.inputs[index] == fi.inputs[np];
+        reveal MapMatchesSeqs();
+        reveal SeqsToMap();
+        assert fi_next.inputs[np] == si.inputs[index];
+      }
+      assert fi_next.inputs == fi.inputs;
+
+      assert fi_next.state == SeqsToMap(state, si.state);
+      forall n | n in fi.state
+        ensures fi_next.state[n] == fi.state[n]
+      {
+        reveal Seq.ToSet();
+        assert n in state;
+        var index := Seq.IndexOf(state, n);
+        assert si.state[index] == fi.state[n];
+        reveal MapMatchesSeqs();
+        reveal SeqsToMap();
+        assert fi_next.state[n] == si.state[index];
+      }
+      assert fi_next.inputs == fi.inputs;
+    }
+
+    lemma fo2so2fo(fo: FO)
+      requires Valid()
+      requires FOValid(fo, outputs, state)
+      ensures so2fo(fo2so(fo)) == fo
+    {
+      var so := fo2so(fo);
+      assert so.outputs == seq(|outputs|, (index: nat) requires index < |outputs| =>
+        reveal Seq.ToSet();
+        fo.outputs[outputs[index]]);
+      var fo_next := so2fo(so);
+      assert fo_next.outputs == SeqsToMap(outputs, so.outputs);
+      forall np | np in fo.outputs
+        ensures fo_next.outputs[np] == fo.outputs[np]
+      {
+        reveal Seq.ToSet();
+        assert np in outputs;
+        var index := Seq.IndexOf(outputs, np);
+        assert so.outputs[index] == fo.outputs[np];
+        reveal MapMatchesSeqs();
+        reveal SeqsToMap();
+        assert fo_next.outputs[np] == so.outputs[index];
+      }
+      assert fo_next.outputs == fo.outputs;
+
+      assert fo_next.state == SeqsToMap(state, so.state);
+      forall n | n in fo.state
+        ensures fo_next.state[n] == fo.state[n]
+      {
+        reveal Seq.ToSet();
+        assert n in state;
+        var index := Seq.IndexOf(state, n);
+        assert so.state[index] == fo.state[n];
+        reveal MapMatchesSeqs();
+        reveal SeqsToMap();
+        assert fo_next.state[n] == so.state[index];
+      }
+      assert fo_next.outputs == fo.outputs;
+    }
+
+    lemma si2fi2si(si: SI)
+      requires Valid()
+      requires SIValid(si, inputs, state)
+      ensures fi2si(si2fi(si)) == si
+    {
+      reveal MapMatchesSeqs();
+      reveal SeqsToMap();
+    }
+
+    lemma so2fo2so(so: SO)
+      requires Valid()
+      requires SOValid(so, outputs, state)
+      ensures fo2so(so2fo(so)) == so
+    {
+      reveal MapMatchesSeqs();
+      reveal SeqsToMap();
+    }
+
+    //function f(fi: FI): (fo: FO)
+    //  requires Valid()
+    //  requires FIValid(fi, inputs, state)
+    //  ensures FOValid(fo, outputs, state)
+    //{
+    //  var si := fi2si(fi);
+    //  assert SIValid(si, inputs, state);
+    //  //reveal Valid();
+    //  var so := sf(si);
+    //  var fo := so2fo(so);
+    //  fo
+    //}
+
   }
 
-  datatype RFunction = RFunction(
+  predicate ScufMapUpdateFunctionConsistent(mp: ScufMap, uf: UpdateFunction)
+    requires mp.Valid()
+    requires uf.Valid()
+  {
+    && (|mp.inputs| == uf.input_width)
+    && (|mp.outputs| == uf.output_width)
+    && (|mp.state| == uf.state_width)
+  }
+
+  //opaque ghost predicate MapFunctionsEquiv(mf1: MapFunction, mf2: MapFunction)
+  //  requires mf1.Valid()
+  //  requires mf2.Valid()
+  //{
+  //  reveal MapFunction.Valid();
+  //  && mf1.inputs == mf2.inputs
+  //  && mf1.outputs == mf2.outputs
+  //  && mf1.state == mf2.state
+  //  && forall fi: FI :: FIValid(fi, mf1.inputs, mf1.state) ==> (
+  //    mf1.f(fi) == mf2.f(fi)
+  //  )
+  //}
+
+  //opaque ghost predicate MapFunctionsSFEquiv(mf1: MapFunction, mf2: MapFunction)
+  //  requires mf1.Valid()
+  //  requires mf2.Valid()
+  //{
+  //  reveal MapFunction.Valid();
+  //  && mf1.inputs == mf2.inputs
+  //  && mf1.outputs == mf2.outputs
+  //  && mf1.state == mf2.state
+  //  && forall si: SI :: SIValid(si, mf1.inputs, mf1.state) ==> (
+  //    mf1.sf(si) == mf2.sf(si)
+  //  )
+  //}
+
+  //lemma MapFunctionsEquivSFEquiv(mf1: MapFunction, mf2: MapFunction)
+  //  requires mf1.Valid()
+  //  requires mf2.Valid()
+  //  requires MapFunctionsSFEquiv(mf1, mf2)
+  //  ensures MapFunctionsEquiv(mf1, mf2)
+  //{
+  //  reveal MapFunctionsSFEquiv();
+  //  reveal MapFunction.Valid();
+  //  forall fi: FI | FIValid(fi, mf1.inputs, mf1.state)
+  //    ensures mf1.f(fi) == mf2.f(fi)
+  //  {
+  //    var si1 := mf1.fi2si(fi);
+  //    var si2 := mf2.fi2si(fi);
+  //    mf1.fi2si2fi(fi);
+  //    mf2.fi2si2fi(fi);
+  //    assert si1 == si2;
+  //    var so1 := mf1.sf(si1);
+  //    var so2 := mf2.sf(si2);
+  //    assert so1 == so2;
+  //    var fo1 := mf1.f(fi);
+  //    var fo2 := mf2.f(fi);
+  //    assert fo1 == mf1.so2fo(so1);
+  //    assert fo2 == mf2.so2fo(so2);
+  //    assert fo1 == fo2;
+  //  }
+  //  reveal MapFunctionsEquiv();
+  //}
+
+  datatype UpdateFunction = UpdateFunction(
     input_width: nat,
     output_width: nat,
     state_width: nat,
@@ -518,68 +670,79 @@ module MapFunction {
       reveal Valid();
     }
 
-    opaque ghost predicate MFConsistent(mf: MapFunction)
-      requires Valid()
-    {
-      reveal Valid();
-      && (|mf.inputs| == input_width)
-      && (|mf.outputs| == output_width)
-      && (|mf.state| == state_width)
-      && (forall si :: SIVal(si) ==> mf.sf.requires(si) && mf.sf(si) == sf(si))
-    }
+    //opaque ghost predicate MFConsistent(mf: MapFunction)
+    //  requires Valid()
+    //{
+    //  reveal Valid();
+    //  && (|mf.inputs| == input_width)
+    //  && (|mf.outputs| == output_width)
+    //  && (|mf.state| == state_width)
+    //  && (forall si :: SIVal(si) ==> mf.sf.requires(si) && mf.sf(si) == sf(si))
+    //}
 
-    function ReplacementMF(old_mf: MapFunction): (new_mf: MapFunction)
-      requires Valid()
-      requires old_mf.Valid()
-      requires MFConsistent(old_mf)
-      ensures new_mf.Valid()
-      ensures MapFunctionsEquiv(old_mf, new_mf)
-      ensures MFConsistent(new_mf)
-    {
-      reveal Valid();
-      reveal MapFunction.Valid();
-      reveal MFConsistent();
-      reveal MapFunctionsEquiv();
-      MapFunction(
-        old_mf.inputs,
-        old_mf.outputs,
-        old_mf.state,
-        (si: SI) requires SIVal(si) => sf(si)
-      )
-    }
+    //function ReplacementMF(old_mf: MapFunction): (new_mf: MapFunction)
+    //  requires Valid()
+    //  requires old_mf.Valid()
+    //  requires MFConsistent(old_mf)
+    //  ensures new_mf.Valid()
+    //  ensures MapFunctionsEquiv(old_mf, new_mf)
+    //  ensures MFConsistent(new_mf)
+    //{
+    //  reveal Valid();
+    //  reveal MapFunction.Valid();
+    //  reveal MFConsistent();
+    //  reveal MapFunctionsEquiv();
+    //  MapFunction(
+    //    old_mf.inputs,
+    //    old_mf.outputs,
+    //    old_mf.state,
+    //    (si: SI) requires SIVal(si) => sf(si)
+    //  )
+    //}
   }
 
-  opaque ghost predicate RFunctionEquiv(rf1: RFunction, rf2: RFunction)
+  opaque ghost predicate UpdateFunctionsEquiv(rf1: UpdateFunction, rf2: UpdateFunction)
     requires rf1.Valid()
     requires rf2.Valid()
   {
-    reveal RFunction.Valid();
+    reveal UpdateFunction.Valid();
     && rf1.input_width == rf2.input_width
     && rf1.output_width == rf2.output_width
     && rf1.state_width == rf2.state_width
     && (forall si: SI :: rf1.SIVal(si) ==> rf1.sf(si) == rf2.sf(si))
   }
 
-  lemma MFConsistentEquiv(rf1: RFunction, rf2: RFunction, mf: MapFunction)
-    requires rf1.Valid()
-    requires rf2.Valid()
-    requires mf.Valid()
-    requires RFunctionEquiv(rf1, rf2) || RFunctionEquiv(rf2, rf1)
-    requires rf1.MFConsistent(mf)
-    ensures rf2.MFConsistent(mf)
+  lemma UFConsistentEquiv(uf1: UpdateFunction, uf2: UpdateFunction, mp: ScufMap) 
+    requires uf1.Valid()
+    requires uf2.Valid()
+    requires mp.Valid()
+    requires UpdateFunctionsEquiv(uf1, uf2) || UpdateFunctionsEquiv(uf2, uf1)
+    requires ScufMapUpdateFunctionConsistent(mp, uf1)
+    ensures ScufMapUpdateFunctionConsistent(mp, uf2)
   {
-    reveal RFunctionEquiv();
-    reveal RFunction.MFConsistent();
+    reveal UpdateFunctionsEquiv();
   }
 
-  const NullMF := MapFunction(
-    [], [], [],
+  //const NullMF := MapFunction(
+  //  [], [], [],
+  //  (si: SI) requires |si.inputs| == 0 && |si.state| == 0 => SO([], []))
+
+  const NullScufMap := ScufMap([], [], [])
+
+  lemma NullScufMapValid()
+    ensures NullScufMap.Valid()
+  {
+    reveal Seq.HasNoDuplicates();
+    reveal Seq.ToSet();
+  }
+
+  const NullUpdateFunction := UpdateFunction(0, 0, 0,
     (si: SI) requires |si.inputs| == 0 && |si.state| == 0 => SO([], []))
 
-  lemma NullMFValid()
-    ensures NullMF.Valid()
+  lemma NullUpdateFunctionValid()
+    ensures NullUpdateFunction.Valid()
   {
-    reveal MapFunction.Valid();
+    reveal UpdateFunction.Valid();
     reveal Seq.ToSet();
     reveal Seq.HasNoDuplicates();
   }
@@ -604,12 +767,12 @@ module MapFunction {
     }
   }
 
-  ghost predicate RFWillOutput(rf: RFunction, delay: nat, state: seq<bool>, bo: seq<bool>)
+  ghost predicate RFWillOutput(rf: UpdateFunction, delay: nat, state: seq<bool>, bo: seq<bool>)
     requires rf.Valid()
     requires |bo| == rf.output_width
     requires |state| == rf.state_width
   {
-    reveal RFunction.Valid();
+    reveal UpdateFunction.Valid();
     forall si :: rf.SIVal(si) && si.state == state ==> (
       if delay == 0 then
         rf.sf(si).outputs == bo
@@ -619,11 +782,11 @@ module MapFunction {
     )
   } 
 
-  ghost predicate DelayREquiv(df: DelayFunction, rf: RFunction)
+  ghost predicate DelayREquiv(df: DelayFunction, rf: UpdateFunction)
     requires df.Valid()
     requires rf.Valid()
   {
-    reveal RFunction.Valid();
+    reveal UpdateFunction.Valid();
     && (df.input_width == rf.input_width)
     && (df.output_width == rf.output_width)
     && (forall si :: rf.SIVal(si) ==>
